Test/allocated1/dafny0/Twostate-Functions.dfy
@@ -7,31 +7,31 @@ module Basic {
     var bb: int
     var next: U?
 
-    static twostate ghost function H0(new u: U): int
+    static twostate function H0(new u: U): int
       requires allocated(u) && 10 <= old(u.aa)  // error: u is not available in the old state
     {
       5
     }
 
-    static twostate ghost function H1(new u: U): int
+    static twostate function H1(new u: U): int
       requires allocated(u)
     {
       old(u.aa)  // error: u is not available in the old state
     }
 
-    twostate ghost function K0(u: U): int
+    twostate function K0(u: U): int
       requires allocated(u)
     {
       u.aa  // error: reads clause must include u
     }
 
-    twostate ghost function K1(u: U): int
+    twostate function K1(u: U): int
       requires allocated(u) && old(allocated(u))
     {
       old(u.aa)  // note, no reads clause needed to read the old state
     }
 
-    twostate ghost predicate R(u: U)
+    twostate predicate R(u: U)
       requires allocated(u) && old(allocated(u)) && 10 <= old(u.aa)
       reads u
       ensures u.aa < old(u.aa) < 50 ==> R(u)
@@ -39,7 +39,7 @@ module Basic {
       u.aa + old(u.aa) < 100
     }
 
-    twostate ghost function GG<T>(x: int, new t: T): real
+    twostate function GG<T>(x: int, new t: T): real
       requires old(aa) <= aa && unchanged(`bb)
       reads this
       ensures old(aa) <= aa && bb == old(bb)
@@ -51,7 +51,7 @@ module Basic {
         x as real
     }
 
-    twostate ghost predicate AIsIncreased()
+    twostate predicate AIsIncreased()
       reads this
     {
       old(aa) < aa
@@ -96,12 +96,12 @@ module Basic {
       ghost var x := K0(u);  // error: u is not new
     }
 
-    twostate ghost function Sw0(n: nat, x: U, new y: U): real
+    twostate function Sw0(n: nat, x: U, new y: U): real
     {
       if n == 0 then 8.29 else Sw0(n-1, y, x)  // error: parameter 1 is not new enough
     }
 
-    twostate ghost function Sw1(n: nat, x: U, new y: U): real
+    twostate function Sw1(n: nat, x: U, new y: U): real
       requires x == y
     {
       if n == 0 then 8.29 else Sw1(n-1, y, x)  // error under /allocated:1
@@ -113,12 +113,12 @@ module M0 {
   class C {
     var data: nat
   }
-  twostate ghost function F(x: int, c: C, new d: C): int
+  twostate function F(x: int, c: C, new d: C): int
     requires allocated(c) && allocated(d)
     reads c, d
 
   trait Tr {
-    twostate ghost function G(c: C?, new d: C): int
+    twostate function G(c: C?, new d: C): int
       requires c != null && old(allocated(c)) && unchanged(c)
       reads c, d
       ensures old(c.data) <= G(c, d)
@@ -127,7 +127,7 @@ module M0 {
       ensures old(c.data) <= G(c, d)
   }
   class Cl extends Tr {
-    twostate ghost function G(c: C?, new d: C): int
+    twostate function G(c: C?, new d: C): int
       requires c != null && allocated(c) ==> c.data <= old(c.data)  // error under /allocated:1 (c dereferenced inside old)
       reads c
       ensures c != null && allocated(c) ==> G(c, d) == c.data  // error under /allocated:1 (c passed as old parameter to G)
@@ -144,7 +144,7 @@ module M0 {
 }
 
 module M1 refines M0 {
-  twostate ghost function F...
+  twostate function F...
   {
     x +
       old(c.data) +
@@ -157,7 +157,7 @@ module M1 refines M0 {
 module Hof {
   class D {
     var data: int
-    twostate ghost function P(d: D): int
+    twostate function P(d: D): int
       requires allocated(d)
       reads d
     {
@@ -177,8 +177,8 @@ module Hof {
         x := p(e);  // fine
       }
     }
-    // same thing as above, but with a static two-state ghost function and method
-    static twostate ghost function Q(d: D): int
+    // same thing as above, but with a static two-state function and method
+    static twostate function Q(d: D): int
       requires allocated(d)
       reads d
     {
